src/Init/Data/UInt/Bitwise.lean
@@ -9,17 +9,24 @@ import Init.Data.Fin.Bitwise
 import Init.Data.BitVec.Lemmas
 
 set_option hygiene false in
-macro "declare_bitwise_uint_theorems" typeName:ident : command =>
+macro "declare_bitwise_uint_theorems" typeName:ident bits:term:arg : command =>
+let toNat_and := Lean.mkIdentFrom typeName (typeName.getId.modifyBase (·.str "toNat_and"))
 `(
 namespace $typeName
 
-@[simp] protected theorem and_toNat (a b : $typeName) : (a &&& b).toNat = a.toNat &&& b.toNat := BitVec.toNat_and ..
+@[simp] protected theorem toNat_and (a b : $typeName) : (a &&& b).toNat = a.toNat &&& b.toNat := BitVec.toNat_and ..
+@[simp] protected theorem toNat_or (a b : $typeName) : (a ||| b).toNat = a.toNat ||| b.toNat := BitVec.toNat_or ..
+@[simp] protected theorem toNat_xor (a b : $typeName) : (a ^^^ b).toNat = a.toNat ^^^ b.toNat := BitVec.toNat_xor ..
+@[simp] protected theorem toNat_shiftLeft (a b : $typeName) : (a <<< b).toNat = a.toNat <<< (b.toNat % $bits) % 2 ^ $bits := BitVec.toNat_shiftLeft
+@[simp] protected theorem toNat_shiftRight (a b : $typeName) : (a >>> b).toNat = a.toNat >>> (b.toNat % $bits) := BitVec.toNat_ushiftRight ..
+
+@[deprecated $toNat_and (since := "2024-11-23")] protected theorem and_toNat (a b : $typeName) : (a &&& b).toNat = a.toNat &&& b.toNat := BitVec.toNat_and ..
 
 end $typeName
 )
 
-declare_bitwise_uint_theorems UInt8
-declare_bitwise_uint_theorems UInt16
-declare_bitwise_uint_theorems UInt32
-declare_bitwise_uint_theorems UInt64
-declare_bitwise_uint_theorems USize
+declare_bitwise_uint_theorems UInt8 8
+declare_bitwise_uint_theorems UInt16 16
+declare_bitwise_uint_theorems UInt32 32
+declare_bitwise_uint_theorems UInt64 64
+declare_bitwise_uint_theorems USize System.Platform.numBits
